partial/Exception.v
@@ -88,7 +88,7 @@ Inductive VM : Conf -> Conf -> Prop :=
 where "x ==> y" := (VM x y).
 
 Inductive cle : Conf -> Conf -> Prop :=
- | cle_mem  f s s' : s ≤ s' -> cle (f, s) (f, s').
+ | cle_mem  f s s' : s ⊑ s' -> cle (f, s) (f, s').
 
 Hint Constructors cle.
 
@@ -158,7 +158,7 @@ Proof.
                 end
     | None => ⟪h, s⟫
     end.
-  ≤ { auto }
+  ⊑ { auto }
     match eval e1 with
     | Some n => match eval e2 with
                 | Some n' => ⟨c , n + n' ,h, s[r:=VAL n]⟩
@@ -221,7 +221,7 @@ Proof.
       | Some n => ⟨c , n ,h, s⟩
       | None => ⟨comp e2 r c, 0 ,h, s⟩
       end.
-  ≤ { eauto }
+  ⊑ { eauto }
       match eval e1 with
       | Some n => ⟨c , n ,h, s⟩
       | None => ⟨comp e2  r c , 0 ,h, s[r:= HAN h]⟩
@@ -231,7 +231,7 @@ Proof.
       | Some n => ⟨c, n, h, s⟩
       | None => ⟪(comp e2 r c,r), s[r:= HAN h]⟫
       end.
-  ≤ {auto}
+  ⊑ {auto}
       match eval e1 with
       | Some n => ⟨c, n, h, s[r:= HAN h]⟩
       | None => ⟪(comp e2 r c,r), s[r:= HAN h]⟫
