partial/LocalState.v
@@ -103,7 +103,7 @@ where "x ==> y" := (VM x y).
 
 
 Inductive cle : Conf -> Conf -> Prop :=
- | cle_mem  f s s' : s ≤ s' -> cle (f, s) (f, s').
+ | cle_mem  f s s' : s ⊑ s' -> cle (f, s) (f, s').
 
 Hint Constructors cle.
 
@@ -172,7 +172,7 @@ Proof.
                       end
     | None => ⟪p, s⟫
     end.
-  ≤ { auto }
+  ⊑ { auto }
     match eval e1 q with
     | Some (n, q') => match eval e2 q' with
                       | Some (n', q'') => ⟨c , n + n' ,p, q'', s[r:=VAL n]⟩
@@ -235,7 +235,7 @@ Proof.
       | Some (n, q') => ⟨c, n ,p, q', s⟩
       | None => ⟨comp' e2  r c , 0 ,p, q, s⟩
       end.
-  ≤ { eauto }
+  ⊑ { eauto }
       match eval e1 q with
       | Some (n, q') => ⟨c , n ,p, q', s⟩
       | None => ⟨comp' e2  r c , 0 ,p, q, s[r:= HAN (comp' e2  r c) p q]⟩
@@ -245,7 +245,7 @@ Proof.
       | Some (n, q') => ⟨c , n ,p, q', s⟩
       | None => ⟪Some r, s[r:= HAN (comp' e2  r c) p q]⟫
       end.
-  ≤ {auto}
+  ⊑ {auto}
       match eval e1 q with
       | Some (n, q') => ⟨c , n ,p, q', s[r:= HAN (comp' e2  r c) p q]⟩
       | None => ⟪Some r, s[r:= HAN (comp' e2  r c) p q]⟫
